theories/Secure/SecureEqProgInsensFacts.v
@@ -1,0 +1,106 @@
+From Coq Require Import
+     Arith.PeanoNat
+     Lists.List
+     Strings.String
+     Morphisms
+     Setoid
+     RelationClasses
+     Logic.Classical_Prop
+     Logic.EqdepFacts
+     Program.Equality
+.
+
+From ExtLib Require Import
+     Data.String
+     Structures.Monad
+     Structures.Traversable
+     Data.List.
+
+From ITree Require Import
+     ITree
+     ITreeFacts
+     Basics.HeterogeneousRelations
+     Events.MapDefault
+     Events.State
+     Events.StateFacts
+     Core.Divergence
+     Dijkstra.TracesIT
+     Secure.SecureEqHalt
+     Secure.SecureEqProgInsens
+.
+
+From Paco Require Import paco.
+
+Import Monads.
+Import MonadNotation.
+Local Open Scope monad_scope.
+
+Variant case_rel {A1 A2 B : Type} (R1 : A1 -> B -> Prop) (R2 : A2 -> B -> Prop) : (A1 + A2) -> B -> Prop :=
+  | crl a1 b : R1 a1 b -> case_rel R1 R2 (inl a1) b
+  | crr a2 b : R2 a2 b -> case_rel R1 R2 (inr a2) b.
+
+Lemma pi_eqit_secure_iter_ret E R S1 S2 Label priv l b2 s body
+      (Rinv : R -> S2 -> Prop) (RS : S1 -> S2 -> Prop)
+  (HRinv : (forall r', Rinv r' s ->
+            pi_eqit_secure Label priv (case_rel Rinv RS) true b2 l (body r') (Ret s) )) :
+  forall r,
+  Rinv r s ->
+  @pi_eqit_secure E S1 S2 Label priv RS true b2 l (ITree.iter body r) (Ret s).
+Proof.
+  ginit. gcofix CIH. intros r0 Hr0. setoid_rewrite unfold_iter.
+  assert (pi_eqit_secure Label priv (case_rel Rinv RS) true b2 l (body r0) (Ret s)).
+  auto. remember (body r0) as t. clear Heqt. generalize dependent t.
+  gcofix CIH'. intros t Ht.
+  destruct (observe t) eqn : Heq; symmetry in Heq; apply simpobs in Heq.
+  - rewrite Heq.
+    assert (pi_eqit_secure Label priv (case_rel Rinv RS) true b2 l (Ret r1) (Ret s) ).
+    rewrite <- Heq. auto.
+    pinversion H. subst. inv H2.
+    + rewrite bind_ret_l. gstep. constructor; auto.
+      gfinal. left. eapply CIH; eauto.
+    + rewrite bind_ret_l. gstep. constructor. auto.
+  - rewrite Heq. rewrite bind_tau. gstep. constructor; auto.
+    gfinal. left. eapply CIH'.
+    assert (pi_eqit_secure Label priv (case_rel Rinv RS) true b2 l (Tau t0) (Ret s)).
+    rewrite <- Heq. auto. pinversion H. rewrite <- itree_eta. auto.
+  - destruct (classic (leq (priv _ e) l ) ).
+    + exfalso. apply HRinv in Hr0.
+      assert (pi_eqit_secure Label priv (case_rel Rinv RS) true b2 l (Vis e k) (Ret s) ).
+      { rewrite <- Heq. auto. }
+      pinversion H0; subst. ITrace.inj_existT. subst. contradiction.
+    + rewrite Heq. rewrite bind_vis.
+      gstep. constructor; auto. intros x. gfinal. left. eapply CIH'.
+      assert ( pi_eqit_secure Label priv (case_rel Rinv RS) true b2 l (Vis e k) (Ret s)) .
+      rewrite <- Heq. auto. pinversion H0; subst; ITrace.inj_existT; subst.
+      rewrite <- itree_eta. apply H2.
+Qed.
+
+Ltac use_simpobs :=
+  repeat match goal with 
+         | H : TauF _ = observe ?t |- _ => apply simpobs in H 
+         | H : RetF _ = observe ?t |- _ => apply simpobs in H
+         | H : VisF _ _ = observe ?t |- _ => apply simpobs in H
+  end.
+
+(* I believe we could generalize this lemma for any t2 that converges along all paths *)
+Lemma pi_eqit_secure_trans_ret E R1 R2 R3 Label priv l b1 b2 
+      (RR1 : R1 -> R2 -> Prop) (RR2 : R2 -> R3 -> Prop) 
+      (t1 : itree E R1) (r : R2) (t3 : itree E R3) :
+  pi_eqit_secure Label priv RR1 b1 b2 l t1 (Ret r) ->
+  pi_eqit_secure Label priv RR2 b1 b2 l (Ret r) t3 ->
+  pi_eqit_secure Label priv (rcompose RR1 RR2) b1 b2 l t1 t3.
+Proof.
+  revert t1 t3. ginit. gcofix CIH.
+  intros. pinversion H0; subst; try inv CHECK; use_simpobs.
+  - rewrite H. generalize dependent t3. gcofix CIH'. intros t3 Ht3.
+    pinversion Ht3; use_simpobs.
+    + rewrite H2. gstep. constructor; auto. econstructor; eauto.
+    + rewrite H2. gstep. constructor; auto. gfinal. left. eapply CIH'.
+      symmetry in H1. use_simpobs. rewrite H1 in H4. auto.
+    + rewrite H2. gstep. constructor; auto. intros. gfinal. left.
+      eapply CIH'. symmetry in H1. use_simpobs. setoid_rewrite H1 in H4. apply H4.
+  - symmetry in H2. use_simpobs. rewrite H. gstep. constructor; auto.
+    gfinal. left. eapply CIH; auto. rewrite <- H2. auto.
+  - symmetry in H2. use_simpobs. rewrite H. gstep. constructor; auto.
+    intros. gfinal. left. apply CIH; auto. rewrite <- H2. apply H3.
+Qed.
