theories/Secure/SecurityImpExc/SecurityImpTypesProgInsens.v
@@ -1,0 +1,505 @@
+From Coq Require Import
+     Arith.PeanoNat
+     Lists.List
+     Strings.String
+     Morphisms
+     Setoid
+     RelationClasses
+     Logic.Classical_Prop
+.
+
+From ExtLib Require Import
+     Data.String
+     Structures.Monad
+     Structures.Traversable
+     Data.List.
+
+From ITree Require Import
+     ITree
+     ITreeFacts
+     HeterogeneousRelations
+     Events.MapDefault
+     Events.State
+     Events.StateFacts
+     Events.Exception
+     Events.ExceptionFacts
+     Core.Divergence
+     Dijkstra.TracesIT
+     Dijkstra.ITrace
+     Secure.SecureEqHalt
+     Secure.SecurityImpExc.SecurityImp
+     Secure.SecurityImpExc.SecurityImpHandler
+     Secure.SecurityImpExc.RaiseException
+     Secure.SecureEqProgInsens
+     Secure.SecureEqProgInsensFacts
+.
+
+From ITree Require Import 
+     Secure.SecurityImpExc.SecurityImpTypes.
+
+Import Monads.
+Import MonadNotation.
+Local Open Scope monad_scope.
+Local Open Scope string_scope.
+
+Instance sense_preorder_in : Preorder := sense_preorder.
+
+Notation label := sensitivity.
+
+Definition labelled_equiv  :=
+  SecurityImpTypes.labelled_equiv.
+
+Instance labelled_equit_equiv {Γ l} : Equivalence (labelled_equiv Γ l).
+Proof.
+  constructor; unfold labelled_equiv.
+  - red. red. intros; auto.
+  - do 2 red. intros. symmetry; auto.
+  - do 2 red. intros. rewrite H; auto.
+Qed.
+
+Definition label_pi_eqit_secure_impstate  (b1 b2 : bool) (Γ : privacy_map) (l : label) {R1 R2 : Type} (RR : R1 -> R2 -> Prop )
+           (m1 : stateT map (itree (impExcE +' IOE)) R1) (m2 : stateT map (itree (impExcE +' IOE)) R2) : Prop :=
+  forall σ1 σ2, labelled_equiv Γ l σ1 σ2 -> pi_eqit_secure sense_preorder priv_exc_io (product_rel (labelled_equiv Γ l) RR) b1 b2 l (m1 σ1) (m2 σ2).
+
+Definition label_state_pi_sec_eutt {R1 R2} priv l (RR : R1 -> R2 -> Prop) m1 m2 :=
+  label_pi_eqit_secure_impstate true true  priv l RR m1 m2.
+
+Definition sem_stmt (s : stmt) := interp_imp (denote_stmt s).
+
+Definition sem_throw_stmt (s : stmt) := interp_imp (throw_prefix (denote_stmt s) ).
+
+Definition sem_expr (e : expr) := SecurityImpTypes.sem_expr e.
+
+Definition state_equiv {E R} (m1 m2 : stateT map (itree E) R) := forall (σ : map), m1 σ ≈ m2 σ.
+
+Locate pi_eqit_secure.
+
+Global Instance proper_eutt_pi_secure_eutt  {E R1 R2 RR Label priv l} : Proper (@eutt E R1 R1 eq ==> @eutt E R2 R2 eq ==> Basics.flip Basics.impl)
+                                                               (pi_eqit_secure Label priv RR true true l).
+Proof.
+Admitted.
+
+Global Instance proper_eq_itree_secure_eutt  {E R1 R2 RR Label priv l} : Proper (@eq_itree E R1 R1 eq ==> @eq_itree E R2 R2 eq ==> Basics.flip Basics.impl)
+                                                               (pi_eqit_secure Label priv RR true true l).
+Proof.
+  repeat intro. assert (x ≈ y). rewrite H. reflexivity. 
+  assert (x0 ≈ y0). rewrite H0. reflexivity. setoid_rewrite H3. rewrite H2. auto.
+Qed.
+
+Global Instance proper_state_equiv_label_state_sec_eutt {R1 R2 RR priv l} : Proper (@state_equiv _ R1 ==> @state_equiv _ R2 ==> iff) (@label_state_pi_sec_eutt R1 R2 priv l RR).
+Proof.
+  repeat intro. split.
+  - intros. do 2 red in H1. do 2 red. intros. red in H0. specialize (H0 σ2). red in H.
+    specialize (H σ1). eapply proper_eutt_pi_secure_eutt; eauto. symmetry. auto. symmetry. auto.
+  - intros. intros. do 2 red in H1. do 2 red. intros. red in H0. specialize (H0 σ2). red in H.
+    specialize (H σ1).  eapply proper_eutt_pi_secure_eutt; eauto.
+Qed.
+
+Context (Γ : privacy_map).
+
+Variant secure_stmt_at_label (observer pc lexn : label) (s : stmt) : Prop :=
+  | ssal_leq : (leq pc observer) -> label_state_pi_sec_eutt Γ observer eq (sem_stmt s) (sem_stmt s) -> secure_stmt_at_label observer pc lexn s
+  | ssal_nleq : (~ leq pc observer) -> label_state_pi_sec_eutt Γ observer top2 (sem_stmt s) (ret tt) -> secure_stmt_at_label observer pc lexn s.
+
+
+
+Variant secure_expr_at_label (observer protection: label ) (e : expr) : Prop :=
+  | seal_leq : (leq protection observer) -> label_state_pi_sec_eutt Γ observer eq (sem_expr e) (sem_expr e) -> 
+               secure_expr_at_label observer protection e
+  | seal_nleq : (~leq protection observer) -> (exists n:value, label_state_pi_sec_eutt Γ observer top2 (sem_expr e) (ret n)) ->
+                secure_expr_at_label observer protection e
+.
+
+Definition secure_expr l e := forall observer, secure_expr_at_label observer l e.
+
+Definition secure_stmt pc lexn s := forall observer, secure_stmt_at_label observer pc lexn s.
+
+Variant is_inl {A B : Type} : A + B -> Prop :=
+  | is_inl_ev (a : A) : is_inl (inl a).
+
+
+(* I need cases like rsense_termlexcr so for when public observers look at private 
+   exceptions throw the sum type lense *)
+Variant Rsense (observer lexn : label) : unit + label -> unit + label -> Prop :=
+  | rsense_termlr : Rsense observer lexn (inl tt) (inl tt)
+  | rsense_exclr l1 l2 : leq l1 lexn -> leq l2 lexn -> Rsense observer lexn (inr l1) (inr l2)
+  | rsense_termlexcr lpriv : leq lpriv lexn -> ~ leq lpriv observer -> Rsense observer lexn (inl tt) (inr lpriv)
+  | rsense_excltermr lpriv : leq lpriv lexn -> ~ leq lpriv observer -> Rsense observer lexn (inr lpriv) (inl tt)
+.
+
+Instance sym_rsense {observer lexn} : Symmetric (Rsense observer lexn).
+Proof.
+  red. intros. inv H; constructor; auto.
+Qed.
+
+Variant secure_throw_stmt_at_label (observer pc lexn : label) (s : stmt) : Prop :=
+  | stsal_leq : leq pc observer -> label_state_pi_sec_eutt Γ observer (Rsense observer lexn )
+                                                       (sem_throw_stmt s) (sem_throw_stmt s) -> secure_throw_stmt_at_label observer pc lexn s
+  | stsal_nleq : (~ leq pc observer) -> label_state_pi_sec_eutt Γ observer (fun sum _ => is_inl sum ) 
+                                                            (sem_throw_stmt s) (ret tt ) ->  secure_throw_stmt_at_label observer pc lexn s
+  .
+(*maybe I can simplify the first return relation, I think some of those conditions are implied by a reasonable secure_stmt def 
+  really what throw_stmt is needed for is the observation of the final state before an exception
+  maybe experiment with the try catch and seq cases, see what is really neededs
+  Intuitively if the exception is visible the labels must be the same (that is certainly true but may be stronger than needed)
+  maybe can get away with just each label is less than lexn1
+  
+*)
+Definition secure_throw_stmt pc lexn s := forall observer, secure_throw_stmt_at_label observer pc lexn s.
+
+Lemma pi_sem_stmt_ret_aux:
+  forall (s2 : stmt) (observer : label) (σ3 σ4 : map),
+    (forall σ1 σ2 : map,
+        labelled_equiv Γ observer σ1 σ2 ->
+        pi_eqit_secure sense_preorder priv_exc_io (product_rel (labelled_equiv Γ observer) top2)
+                       true true observer (sem_stmt s2 σ1) (Ret (σ2, tt))) ->
+    labelled_equiv Γ observer σ3 σ4 ->
+    pi_eqit_secure sense_preorder priv_exc_io (product_rel (labelled_equiv Γ observer) eq) true
+                   true observer (interp_state handle_imp (denote_stmt s2) σ3)
+                   (interp_state handle_imp (denote_stmt s2) σ4).
+Proof.
+  intros s2 observer σ3 σ4 Hσ Hs2.
+  eapply pi_eqit_secure_RR_imp with (RR1 := rcompose  (product_rel (labelled_equiv Γ observer) (@top2 unit unit)) (Basics.flip (product_rel (labelled_equiv Γ observer) top2))).
+  { intros [σ5 [] ] [σ6 [] ] Hr. inv Hr. inv REL1. inv REL2. split; auto.
+    destruct r2 as [σ7 [] ]. etransitivity; eauto. symmetry. auto.
+  }
+  eapply pi_eqit_secure_trans_ret; eauto. 
+  apply pi_eqit_secure_sym. apply Hσ. reflexivity.
+Qed.
+
+Lemma pi_sem_throw_stmt_ret_aux:
+  forall (lexn : label) (s2 : stmt) (observer : label) (σ3 σ4 : map),
+    (forall σ1 σ2 : map,
+        labelled_equiv Γ observer σ1 σ2 ->
+        pi_eqit_secure sense_preorder priv_exc_io
+                       (product_rel (labelled_equiv Γ observer)
+                                    (fun (sum : unit + label) (_ : unit) => is_inl sum)) true true observer
+                       (sem_throw_stmt s2 σ1) (Ret (σ2, tt))) ->
+    labelled_equiv Γ observer σ3 σ4 ->
+    pi_eqit_secure sense_preorder priv_exc_io
+                   (product_rel (labelled_equiv Γ observer) (Rsense observer lexn)) true true
+                   observer (interp_state handle_imp (throw_prefix (denote_stmt s2)) σ3)
+                   (interp_state handle_imp (throw_prefix (denote_stmt s2)) σ4).
+Proof.
+  intros lexn s2 observer σ3 σ4 Hσ H4.
+  set (product_rel (labelled_equiv Γ observer) (fun (sum : unit + label) ( _ : unit) => is_inl sum ) ) as HR.
+  eapply pi_eqit_secure_RR_imp with (RR1 := rcompose HR (Basics.flip HR) ).
+  { unfold HR. intros [σ5 r1] [σ6 r2] Hr. inv Hr. inv REL1. inv REL2.
+    inv H0. inv H2. cbn in H3. cbn in H0. subst.
+    destruct r0 as [σ7 [] ]. split. etransitivity; eauto. symmetry. auto.
+    cbn. destruct a. destruct a0. constructor. }
+  eapply pi_eqit_secure_trans_ret; eauto. apply pi_eqit_secure_sym.
+  eapply Hσ. reflexivity.
+Qed.
+
+Lemma seq_well_typed_correct pc lexn1 lexn2 s1 s2 :
+  secure_stmt pc lexn1 s1 -> secure_stmt (join pc lexn1) lexn2 s2 ->
+  secure_stmt pc (join lexn1 lexn2) (Seq s1 s2).
+Proof.
+  intros Hs1 Hs2 observer.
+  specialize (Hs1 observer). inv Hs1.
+  - left; auto. unfold sem_stmt, interp_imp.
+    cbn. do 2 red. intros σ1 σ2 Hσ. setoid_rewrite interp_state_bind.
+    eapply pi_eqit_secure_bind; eauto. intros [σ3 [] ] [σ4 [] ] [Hσ' _ ].
+    specialize (Hs2 observer). inv Hs2; eauto. cbn. do 2 red in H2. cbn in H2.
+    eapply pi_sem_stmt_ret_aux; eauto.
+  - right; auto. cbn in H0. unfold sem_stmt, interp_imp. cbn.
+    do 2 red. intros σ1 σ2 Hσ.
+    setoid_rewrite <- bind_ret_r with (s := Ret (σ2, tt) ).
+    setoid_rewrite interp_state_bind.
+    eapply pi_eqit_secure_bind; eauto.
+    intros [σ3 [] ] [σ4 [] ] [Hσ' _ ].
+    specialize (Hs2 observer). inv Hs2; eauto.
+    + exfalso. apply H. eapply leq_sense_trans; eauto.
+      apply leq_sense_join_l.
+    + cbn in H2. eauto.
+Qed.
+
+Lemma seq_well_typed_correct' pc lexn1 lexn2 s1 s2 :
+  secure_throw_stmt pc lexn1 s1 -> secure_throw_stmt (join pc lexn1) lexn2 s2 ->
+  secure_throw_stmt pc (join lexn1 lexn2) (Seq s1 s2).
+Proof.
+  intros Hs1 Hs2 observer.
+  specialize (Hs1 observer). inv Hs1.
+  - left; auto. unfold sem_throw_stmt, interp_imp. cbn. do 2 red.
+    intros σ1 σ2 Hσ. setoid_rewrite throw_prefix_bind.
+    setoid_rewrite interp_state_bind.
+    eapply pi_eqit_secure_bind; eauto.
+    intros [σ3 r1] [σ4 r2] [Hσ' Hr]. inv Hr.
+    + specialize (Hs2 observer). inv Hs2; eauto.
+      * cbn.
+        eapply pi_eqit_secure_RR_imp; try eapply H4; eauto.
+        intros. destruct H5. split; auto. inv H6; constructor; auto;
+        try eapply leq_sense_trans; eauto; apply leq_sense_join_r.
+      * cbn in H4. cbn.
+        do 2 red in H4. cbn in Hσ'.
+        eapply pi_sem_throw_stmt_ret_aux; eauto.
+    + setoid_rewrite interp_state_ret. apply pi_eqit_secure_ret.
+      split; auto; constructor; eapply leq_sense_trans; eauto.
+      all : apply leq_sense_join_l.
+    + specialize (Hs2 observer). inv Hs2; eauto.
+      * exfalso. apply H2. eapply leq_sense_trans; eauto.
+        eapply leq_sense_trans; eauto. apply leq_sense_join_r.
+      * setoid_rewrite interp_state_ret. cbn.
+        cbn in H6. do 2 red in H6.
+        match goal with 
+      |- pi_eqit_secure _ _ _ _ _ _ _ ?t => assert (t ≈ ITree.bind (Ret (σ4,tt) ) (fun '(σ',x) => Ret (σ', inr lpriv) )) end.
+        rewrite bind_ret_l. reflexivity.
+        rewrite H7. rewrite <- bind_ret_r.
+        eapply pi_eqit_secure_bind; eauto.
+        intros [σ5 r3] [σ6 r4] [Hσ'' Hr']; inv Hr'.
+        cbn in H8. rewrite <- H8. destruct a. apply pi_eqit_secure_ret.
+        split; auto. constructor; auto. eapply leq_sense_trans; eauto.
+        apply leq_sense_join_l.
+    + specialize (Hs2 observer). inv Hs2; eauto.
+      * exfalso. apply H2. eapply leq_sense_trans; eauto.
+        eapply leq_sense_trans; eauto. apply leq_sense_join_r.
+      * setoid_rewrite interp_state_ret. cbn.
+        cbn in H6.
+        match goal with
+        |- pi_eqit_secure _ _ _ _ _ _ ?t _ => assert (t ≈ ITree.bind (Ret (σ3,tt) ) (fun '(σ',x) => Ret (σ', inr lpriv) )) end.
+        rewrite bind_ret_l. reflexivity. rewrite H7.
+        setoid_rewrite <- bind_ret_r at 4.
+        apply pi_eqit_secure_sym. symmetry in Hσ'. eapply pi_eqit_secure_bind; eauto.
+        intros [σ5 r3] [σ6 [] ] [Hσ'' Hr']; inv Hr'.
+        destruct a. cbn in H8. subst. apply pi_eqit_secure_ret.
+        split; auto. symmetry. auto. constructor; auto.
+        eapply leq_sense_trans; eauto. apply leq_sense_join_l.
+  - right; auto. intros σ1 σ2 Hσ. unfold sem_throw_stmt, interp_imp.
+    cbn. setoid_rewrite throw_prefix_bind. setoid_rewrite interp_state_bind.
+    cbn in H0. rewrite <- bind_ret_r with (s := Ret (σ2, tt) ).
+    eapply pi_eqit_secure_bind; eauto. intros [σ3 r1] [σ4 [] ] [Hσ' Hr]. inv Hr.
+    destruct a. cbn. cbn in H1. subst.
+    specialize (Hs2 observer). inv Hs2.
+    + exfalso. apply H. eapply leq_sense_trans; eauto. apply leq_sense_join_l.
+    + cbn in H2. eauto.
+Qed.
+
+Lemma try_catch_well_typed_correct pc lexn1 lexn2 s1 s2 :
+  secure_stmt pc lexn1 s1 -> secure_throw_stmt pc lexn1 s1 ->
+  secure_stmt (join pc lexn1) lexn2 s2 ->
+  secure_stmt pc lexn2 (TryCatch s1 s2).
+Proof.
+  intros Hs1 Hs1t Hs2 observer.
+  specialize (Hs1 observer). specialize (Hs1t observer).
+  inv Hs1; inv Hs1t; try contradiction.
+  - left; auto. unfold sem_stmt, interp_imp. do 2 red. intros σ1 σ2 Hσ.
+    cbn. setoid_rewrite try_catch_to_throw_prefix.
+    setoid_rewrite interp_state_bind. eapply pi_eqit_secure_bind; eauto.
+    intros [σ3 r1 ] [σ4 r2 ] [Hσ' Hr] ; inv Hr; cbn.
+    + setoid_rewrite interp_state_ret. apply pi_eqit_secure_ret. auto.
+    + specialize (Hs2 observer). inv Hs2; eauto. do 2 red in H8.
+      cbn in H8. eapply pi_sem_stmt_ret_aux; eauto.
+    + specialize (Hs2 observer). inv Hs2. 
+      * exfalso. apply H4. eapply leq_sense_trans; eauto.
+        eapply leq_sense_trans. apply leq_sense_join_r. eauto.
+      * apply pi_eqit_secure_sym. do 2 red in H8.
+        apply pi_eqit_secure_RR_imp with (RR1 := product_rel (labelled_equiv Γ observer) top2).
+        { intros [? [] ] [? [] ] ? . inv H9. split; auto. symmetry. auto. }
+        cbn in H8. setoid_rewrite interp_state_ret. eapply H8. symmetry. auto.
+    + specialize (Hs2 observer). inv Hs2. 
+      * exfalso. apply H4. eapply leq_sense_trans; eauto.
+        eapply leq_sense_trans. apply leq_sense_join_r. eauto.
+      * do 2 red in H8.
+        apply pi_eqit_secure_RR_imp with (RR1 := product_rel (labelled_equiv Γ observer) top2).
+        { intros [? [] ] [? [] ] ? . inv H9. split; auto. }
+        cbn in H8. setoid_rewrite interp_state_ret. eapply H8. auto. 
+  - right; auto. unfold sem_stmt, interp_imp. do 2 red. intros σ1 σ2 Hσ.
+    cbn. setoid_rewrite try_catch_to_throw_prefix.
+    (* rewrite the ret into a trivial bind *)
+    match goal with 
+      |- pi_eqit_secure _ _ _ _ _ _ _ ?t => assert (t ≈ ITree.bind (Ret (σ2,tt) ) (fun x => Ret x)) end.
+    rewrite bind_ret_r. reflexivity. rewrite H3.
+    setoid_rewrite interp_state_bind. cbn in H2.
+    eapply pi_eqit_secure_bind; eauto.
+    intros [σ3 r1] [σ4 [] ] [Hσ' Hr]; inv Hr.
+    destruct a. simpl. setoid_rewrite interp_state_ret.
+    apply pi_eqit_secure_ret. split; cbv; auto.
+Qed.
+
+Lemma try_catch_well_typed_correct' pc lexn1 lexn2 s1 s2 :
+  secure_stmt pc lexn1 s1 -> secure_throw_stmt pc lexn1 s1 ->
+  secure_throw_stmt (join pc lexn1) lexn2 s2 ->
+  secure_throw_stmt pc lexn2 (TryCatch s1 s2).
+Proof.
+  intros Hs1 Hs1t Hs2 observer. specialize (Hs1 observer).
+  specialize (Hs1t observer). inv Hs1; inv Hs1t; try contradiction.
+  - left; auto. unfold sem_throw_stmt, interp_imp. cbn. do 2 red.
+    intros σ1 σ2 Hσ. rewrite throw_prefix_of_try_catch.
+    setoid_rewrite try_catch_to_throw_prefix.
+    setoid_rewrite throw_prefix_bind.
+    repeat setoid_rewrite interp_state_bind. setoid_rewrite bind_bind.
+    eapply pi_eqit_secure_bind; eauto.
+    intros [σ3 r1] [σ4 r2] [Hσ' Hr]; inv Hr; cbn;
+      try setoid_rewrite throw_prefix_ret; try setoid_rewrite interp_state_ret;
+        try setoid_rewrite bind_ret_l; cbn.
+    + setoid_rewrite interp_state_ret. apply pi_eqit_secure_ret.
+      split; auto. constructor.
+    + specialize (Hs2 observer). inv Hs2; eauto.
+      eapply pi_sem_throw_stmt_ret_aux; eauto. 
+    + specialize (Hs2 observer). inv Hs2; eauto.
+      * exfalso. apply H4. eapply leq_sense_trans; eauto.
+        eapply leq_sense_trans; eauto. apply leq_sense_join_r.
+      * apply pi_eqit_secure_sym. cbn in H8. do 2 red in H8.
+        setoid_rewrite interp_state_ret.
+        match goal with
+        |- pi_eqit_secure _ _ _ _ _ _ _ ?t => assert (t ≈ ITree.bind (Ret (σ3, tt) ) (fun '(σ, x) => Ret (σ, inl x) ) ) end.
+        rewrite bind_ret_l. reflexivity. rewrite H9.
+        rewrite <- bind_ret_r. symmetry in Hσ'. eapply pi_eqit_secure_bind; eauto.
+        intros [σ5 r] [σ6 [] ] Hr. inv Hr. inv H11. destruct a. cbn in H12. subst.
+        apply pi_eqit_secure_ret. split. symmetry; auto. constructor.
+    + specialize (Hs2 observer). inv Hs2; eauto.
+      * exfalso. apply H4. eapply leq_sense_trans; eauto.
+        eapply leq_sense_trans; eauto. apply leq_sense_join_r.
+      * setoid_rewrite interp_state_ret.
+         match goal with
+        |- pi_eqit_secure _ _ _ _ _ _ _ ?t => assert (t ≈ ITree.bind (Ret (σ4, tt) ) (fun '(σ, x) => Ret (σ, inl x) ) ) end.
+        rewrite bind_ret_l. reflexivity. rewrite H9. cbn in H8.
+        rewrite <- bind_ret_r. eapply pi_eqit_secure_bind; eauto.
+        intros [σ5 r] [σ6 [] ] Hr. inv Hr. inv H11. destruct a. cbn in H12. subst.
+        apply pi_eqit_secure_ret. split; auto. constructor.
+  - right; auto. unfold sem_throw_stmt, interp_imp. cbn. do 2 red.
+    intros σ1 σ2 Hσ. rewrite throw_prefix_of_try_catch.
+    rewrite try_catch_to_throw_prefix.
+    rewrite throw_prefix_bind. repeat rewrite interp_state_bind.
+    rewrite bind_bind.
+    setoid_rewrite <- bind_ret_r with (s := Ret (σ2, tt) ).
+    cbn in H2.
+    eapply pi_eqit_secure_bind; eauto.
+    intros [σ3 r1] [σ4 r2] [Hσ' Hr]; inv Hr.
+    rewrite throw_prefix_ret, interp_state_ret, bind_ret_l. cbn.
+    rewrite interp_state_ret. apply pi_eqit_secure_ret. split; auto.
+    constructor.
+Qed.
+
+Lemma pi_eqit_secure_while_ret_aux:
+  forall (e : expr) (s : stmt) (observer : label),
+    label_state_pi_sec_eutt Γ observer top2 (sem_stmt s) (ret tt) ->
+    forall σ1 σ2 : map,
+      labelled_equiv Γ observer σ1 σ2 ->
+      pi_eqit_secure sense_preorder priv_exc_io
+                     (product_rel (labelled_equiv Γ observer) top2) true true
+                     observer (sem_stmt (While e s) σ1) (Ret (σ2, tt)).
+Proof.
+  intros e s observer H0 σ1 σ2 H3.
+  unfold sem_stmt, interp_imp.
+  cbn. specialize (@interp_state_iter') as Hisi. red in Hisi. setoid_rewrite Hisi.
+  eapply pi_eqit_secure_iter_ret with (Rinv := product_rel (labelled_equiv Γ observer) eq ).
+  2 : split; auto.
+  intros [σ3 [] ] [Hσ3 _ ]. cbn.
+  setoid_rewrite interp_state_bind. rewrite bind_bind.
+  specialize (expr_only_ret' e σ3) as [n Hn]. setoid_rewrite Hn.
+  rewrite bind_ret_l. destruct n.
+  + cbn. rewrite interp_state_ret, bind_ret_l. cbn. apply pi_eqit_secure_ret.
+    constructor. split; auto. cbv. auto.
+  + cbn. rewrite interp_state_bind. rewrite bind_bind.
+    rewrite <- bind_ret_r with (s0 := Ret (σ2, tt) ). 
+    cbn in H0.
+    eapply pi_eqit_secure_bind; eauto.
+    intros [σ4 [] ] [σ5 [] ] [Hσ' _ ]. rewrite interp_state_ret, bind_ret_l. cbn.
+    apply pi_eqit_secure_ret. constructor. split; auto.
+Qed.
+
+Lemma while_typed_correct e le pc lexn s :
+  secure_expr le e -> secure_stmt (join pc le) lexn s -> secure_stmt pc lexn (While e s).
+Proof.
+  intros He Hs observer.
+  specialize (He observer). specialize (Hs observer).
+  inv Hs; inv He.
+  - left. eapply leq_sense_trans; try apply H. apply leq_sense_join_l.
+    do 2 red. intros σ1 σ2 Hσ. unfold sem_stmt, interp_imp. cbn.
+    specialize (@interp_state_iter') as Hisi. red in Hisi. setoid_rewrite Hisi.
+    apply secure_eqit_iter with (RA := product_rel (labelled_equiv Γ observer) eq );
+      auto.
+    clear σ1 σ2 Hσ. intros [σ1 [] ] [σ2 [] ] [Hσ _ ].
+    cbn. setoid_rewrite interp_state_bind. repeat rewrite bind_bind.
+    eapply pi_eqit_secure_bind; eauto.
+    intros [σ3 v1] [σ4 v2] [Hσ' Hv]; cbn in Hv; subst. cbn.
+    destruct v2.
+    + setoid_rewrite interp_state_ret. setoid_rewrite bind_ret_l.
+      cbn. apply pi_eqit_secure_ret. constructor. auto.
+    + setoid_rewrite interp_state_bind. setoid_rewrite bind_bind. 
+      eapply pi_eqit_secure_bind; eauto.
+      intros [σ5 [] ] [σ6 [] ] [Hσ'' _ ]. setoid_rewrite interp_state_ret.
+      setoid_rewrite bind_ret_l. cbn. apply pi_eqit_secure_ret.
+      constructor; auto.
+  - exfalso. apply H1. eapply leq_sense_trans; eauto. apply leq_sense_join_r.
+  - right. intro. apply H. 
+    (* come up with a lemma for this *)
+    destruct pc; destruct le; destruct observer; cbv; auto.
+    do 2 red. intros. cbn. eapply pi_eqit_secure_while_ret_aux; eauto.
+  - case_leq pc observer.
+    + left; auto. intros σ1 σ2 Hσ.
+      specialize (pi_eqit_secure_while_ret_aux e s observer H0) as Hwhile.
+      eapply pi_sem_stmt_ret_aux; eauto.
+    + right; auto. cbn. do 2 red. intros. eapply pi_eqit_secure_while_ret_aux; eauto.
+Qed.
+
+
+Lemma while_typed_correct' e le pc lexn s : 
+  secure_expr le e -> secure_throw_stmt (join pc le) lexn s -> secure_throw_stmt pc lexn (While e s).
+Proof.
+  intros He Hs observer.
+  specialize (He observer). specialize (Hs observer).
+  inv Hs; inv He.
+  - left. eapply leq_sense_trans; try apply H. apply leq_sense_join_l.
+    do 2 red. intros σ1 σ2 Hσ. unfold sem_throw_stmt, interp_imp. cbn.
+    setoid_rewrite throw_prefix_iter.
+    specialize (@interp_state_iter') as Hisi. red in Hisi. setoid_rewrite Hisi.
+    eapply secure_eqit_iter with (RA := product_rel (labelled_equiv Γ observer) eq ); auto.
+    intros [σ3 [] ] [σ4 [] ] [Hσ' _ ]. cbn. setoid_rewrite throw_prefix_bind.
+    repeat setoid_rewrite interp_state_bind. repeat rewrite bind_bind.
+    setoid_rewrite throw_prefix_denote_expr. setoid_rewrite interp_state_bind.
+    setoid_rewrite bind_bind.
+    eapply pi_eqit_secure_bind; eauto. intros [σ5 v1] [σ6 v2] [Hσ'' Hv]; cbn in Hv; subst.
+    setoid_rewrite interp_state_ret. setoid_rewrite bind_ret_l. cbn.
+    destruct v2; cbn.
+    + setoid_rewrite throw_prefix_ret. tau_steps.
+      apply pi_eqit_secure_ret. constructor. split; auto. constructor.
+    + setoid_rewrite throw_prefix_bind. setoid_rewrite interp_state_bind. 
+      setoid_rewrite bind_bind.
+      eapply pi_eqit_secure_bind; eauto.
+      intros [σ7 r1] [σ8 r2] [Hσ''' Hr]. cbn in Hr. inv Hr.
+      * setoid_rewrite throw_prefix_ret. tau_steps.
+        apply pi_eqit_secure_ret. constructor. split; auto.
+      * tau_steps. apply pi_eqit_secure_ret. constructor. split; auto.
+        constructor; auto.
+      * tau_steps. cbn in Hσ'. cbn in Hσ''. cbn in Hσ'''. admit.
+      * tau_steps. admit.
+
+  - exfalso. apply H1. eapply leq_sense_trans; eauto. apply leq_sense_join_r.
+  - right. intro. apply H.
+    destruct pc; destruct le; destruct observer; cbv; auto.
+    (* need a lemma to relate iter to ret *) admit.
+Abort. 
+
+Inductive well_typed_expr : sensitivity -> expr -> Prop :=
+  | wte_lit l n : well_typed_expr l (Lit n)
+  | wte_var x l : leq (Γ x) l -> well_typed_expr l (Var x)
+  | wte_plus l1 l2 e1 e2 : well_typed_expr l1 e1 -> well_typed_expr l2 e2 ->
+                           well_typed_expr (join l1 l2) (Plus e1 e2)
+  | wte_min l1 l2 e1 e2 : well_typed_expr l1 e1 -> well_typed_expr l2 e2 ->
+                           well_typed_expr (join l1 l2) (Minus e1 e2)
+  | wte_mult l1 l2 e1 e2 : well_typed_expr l1 e1 -> well_typed_expr l2 e2 ->
+                           well_typed_expr (join l1 l2) (Mult e1 e2)
+.
+
+
+(* rework this definition to have only public exceptions*)
+Inductive well_typed_stmt : sensitivity -> sensitivity -> stmt -> Prop :=
+  | wts_manual pc lexn s : secure_stmt pc lexn s /\ secure_throw_stmt pc lexn s -> well_typed_stmt pc lexn s
+  | wts_skip pc : well_typed_stmt pc Public Skip
+  | wts_seq pc lexn1 lexn2 s1 s2 : well_typed_stmt pc lexn1 s1 -> well_typed_stmt (join pc lexn1) lexn2 s2 ->
+                                   well_typed_stmt pc (join lexn1 lexn2) (Seq s1 s2)
+  | wts_assign pc l x e : well_typed_expr l e -> leq (join l pc) (Γ x) ->
+                          well_typed_stmt pc Public (Assign x e)
+  | wts_print pc le lp e : well_typed_expr le e -> leq (join le pc) lp ->
+                           well_typed_stmt pc Public (Output lp e)
+  | wts_if pc le e lexn1 lexn2 s1 s2 : well_typed_expr le e -> well_typed_stmt (join pc le) lexn1 s1 -> well_typed_stmt (join pc le) lexn2 s2 ->
+                                       well_typed_stmt pc (join lexn1 lexn2) (If e s1 s2)
+  | wts_while e le pc lexn s : well_typed_expr le e -> well_typed_stmt (join pc le) lexn s ->
+                         well_typed_stmt pc lexn (While e s)
+  | wts_raise pc lexn : leq pc lexn -> well_typed_stmt pc lexn (Raise lexn)
+  | wts_try pc lexn1 lexn2 s1 s2 : well_typed_stmt pc lexn1 s1 -> well_typed_stmt (join pc lexn1) lexn2 s2 ->
+                                   well_typed_stmt pc lexn2 (TryCatch s1 s2)
+.
